.

theories/Logic/Computer.v
@@ -1,4 +1,5 @@
 Require Import LoL.Prelude.Prelude.
+Require Import LoL.Math.ThN.
 Require Import LoL.Data.Vector.
 
 Section PRIMITIVE_RECURSION. (* Reference: "https://github.com/princeton-vl/CoqGym/blob/master/coq_projects/goedel/primRec.v" *)
@@ -322,6 +323,73 @@ Theorem MuRecsGraph_correct (n : Arity) (m : Arity) (f : MuRecs n m) (xs : Vecto
   : MuRecsGraph f xs z <-> MuRecsSpec n m f xs z.
 Proof.
   pose proof (LEFT := @MuRecsGraph_complete). pose proof (RIGHT := @MuRecsGraph_sound). now firstorder.
+Qed.
+
+Fixpoint MuRecGraph_unique_value (n : Arity) (f : MuRec n) (xs : Vector.t Value n) (z : Value) (z' : Value) (SPEC : MuRecSpec n f xs z) (CALL : MuRecGraph f xs z') {struct SPEC}
+  : z = z'
+with MuRecsGraph_unique_value (n : Arity) (m : Arity) (fs : MuRecs n m) (xs : Vector.t Value n) (z : Vector.t Value m) (z' : Vector.t Value m) (SPEC : MuRecsSpec n m fs xs z) (CALL' : MuRecsGraph fs xs z') {struct SPEC}
+  : z = z'.
+Proof.
+  - destruct SPEC.
+    + exact CALL.
+    + exact CALL.
+    + exact CALL.
+    + simpl in CALL. eapply MuRecGraph_unique_value.
+      * exact SPEC.
+      * destruct CALL as (ys'&CALLs&CALL).
+        assert (claim : ys = ys').
+        { eapply MuRecsGraph_unique_value; [exact g_spec | exact CALLs]. }
+        subst ys'. exact CALL.
+    + simpl in CALL. unfold V.tail in CALL; simpl in CALL. eapply MuRecGraph_unique_value.
+      * eapply SPEC.
+      * exact CALL.
+    + simpl in CALL. destruct CALL as (y&ACC&CALL). unfold V.tail in ACC, CALL; simpl in ACC, CALL.
+      assert (claim : acc = y).
+      { eapply MuRecGraph_unique_value.
+        - exact SPEC1.
+        - exact ACC. 
+      }
+      subst y. eapply MuRecGraph_unique_value.
+      * eapply SPEC2.
+      * exact CALL.
+    + simpl in CALL. destruct CALL as [MIN' CALL].
+      assert (NOT_LT : ~ z < z').
+      { intros LT. pose proof (MIN' z LT) as (p&p_gt_0&CALL').
+        enough (WTS : 0 = p) by lia.
+        eapply MuRecGraph_unique_value.
+        - exact SPEC.
+        - exact CALL'.
+      }
+      assert (NOT_LT' : ~ z' < z).
+      { intros LT. pose proof (MIN z' LT) as (p&p_gt_0&CALL').
+        enough (WTS : p = 0) by lia.
+        eapply MuRecGraph_unique_value. 
+        - exact CALL'.
+        - exact CALL.
+      }
+      lia.
+  - destruct SPEC.
+    + revert z' CALL'. introVNil. i. reflexivity.
+    + revert z' CALL'. introVCons y' ys'. i. simpl in CALL'.
+      destruct CALL' as (y''&ys''&CALL''&CALLs''&EQ). rewrite <- EQ. eapply f_equal2.
+      * eapply MuRecGraph_unique_value; [exact f_spec | exact CALL''].
+      * eapply MuRecsGraph_unique_value; [exact SPEC | exact CALLs''].
+Qed.
+
+Theorem MuRec_isPartialFunction (n : Arity) (f : MuRec n) (xs : Vector.t Value n) (z : Value) (z' : Value)
+  (SPEC : MuRecSpec n f xs z)
+  (SPEC' : MuRecSpec n f xs z')
+  : z = z'.
+Proof.
+  eapply MuRecGraph_unique_value; [exact SPEC | rewrite MuRecGraph_correct; exact SPEC'].
+Qed.
+
+Theorem MuRecs_isPartialFunction (n : Arity) (m : Arity) (fs : MuRecs n m) (xs : Vector.t Value n) (z : Vector.t Value m) (z' : Vector.t Value m)
+  (SPEC : MuRecsSpec n m fs xs z)
+  (SPEC' : MuRecsSpec n m fs xs z')
+  : z = z'.
+Proof.
+  eapply MuRecsGraph_unique_value; [exact SPEC | rewrite MuRecsGraph_correct; exact SPEC'].
 Qed.
 
 End MU_RECURSIVE.
